lean/mettapedia/scripts/prolog/source_term_order_oracle.pl
@@ -1,0 +1,29 @@
+:- initialization(main, main).
+
+emit(Label, Goal, Term) :-
+    once(Goal),
+    term_string(Term, Rendered, [quoted(true), numbervars(true)]),
+    format('~w=~w~n', [Label, Rendered]).
+
+main(_) :-
+    emit(sort_mixed,
+         sort([b,"x",1,1.0,a,b], SortedMixed),
+         SortedMixed),
+    emit(msort_duplicates,
+         msort([b,a,a], MsortedDuplicates),
+         MsortedDuplicates),
+    emit(keysort_stable,
+         keysort([b-0,a-1,a-2], KeysortedStable),
+         KeysortedStable),
+    emit(sort_key_one,
+         sort(1, @=<, [b-0,a-1,a-2], SortedKeyOne),
+         SortedKeyOne),
+    emit(sort_key_two,
+         sort(2, @=<, [b-3,a-1,c-2], SortedKeyTwo),
+         SortedKeyTwo),
+    emit(sort_descending_unique,
+         sort(0, @>, [a,c,b,c], SortedDescendingUnique),
+         SortedDescendingUnique),
+    emit(sort_signed_zero,
+         sort([0.0,-0.0], SortedSignedZero),
+         SortedSignedZero).
